better double neg

FOL.v
@@ -1,10 +1,12 @@
 Require Export syntax.
 
+Reserved Notation "A ⊢ p" (at level 70).
 
 Notation "p ~> q" := (Impl_ _ _ p q) (at level 60).
 Notation "⊥" := (Fal_ _ _).
 Notation "¬ p" := (p ~> ⊥) (at level 60).
 Notation "∀ p ":= (All_ _ _ p) (at level 60).
+
 
 Section implicative.
 
@@ -17,15 +19,16 @@ Section implicative.
     | Impl _ p q => count p + count q
   end.
 
-  Reserved Notation "A |- p" (at level 70).
   Inductive nd_imp (A : list form) : form -> Prop :=
-    | ndHI p : In p A -> A |- p
-    | ndExp p : A |- ⊥ -> A |- p
-    | ndII p q : (p :: A) |- q -> A |- p ~> q
-    | ndIE p q : A |- p ~> q -> A |- p -> A |- q
-  where "A |- p" := (nd_imp A p).
+    | ndHI p : In p A -> A ⊢ p
+    | ndExp p : A ⊢ ⊥ -> A ⊢ p
+    | ndII p q : (p :: A) ⊢ q -> A ⊢ p ~> q
+    | ndIE p q : A ⊢ p ~> q -> A ⊢ p -> A ⊢ q
+  where "A ⊢ p" := (nd_imp A p).
 
-  Lemma weakening_imp A B p : A |- p -> incl A B -> B |- p.
+  Variable nd : list form -> form -> Prop.
+
+  Lemma weakening_imp A B p : A ⊢ p -> incl A B -> B ⊢ p.
   Proof. intro. revert B. induction H; intros B Hinc.
     -apply ndHI. now apply Hinc.
     -apply ndExp. now apply IHnd_imp.
@@ -33,15 +36,10 @@ Section implicative.
     -apply (ndIE _ p). now apply IHnd_imp1. now apply IHnd_imp2.
   Qed.
 
-  Lemma double_neg_imp A p : A |- p -> A |- ¬¬p.
-  Proof. induction 1; apply ndII.
-    -apply (ndIE _ p). { apply ndHI. now left. } { apply ndHI. now right. }
-    -apply (weakening_imp A). assumption. now apply incl_tl.
-    -apply (ndIE _ (p~>q)). { apply ndHI. now left. }
-     apply ndII, (weakening_imp (p::A)). assumption.
-     { apply incl_cons. now left. now repeat apply incl_tl. }
-    -apply (ndIE _ q). { apply ndHI. now left. }
-     apply (weakening_imp A). now apply (ndIE _ p). now apply incl_tl.
+  Lemma double_neg_imp A p : A ⊢ p -> A ⊢ ¬¬p.
+  Proof. apply (ndIE _ p), ndII, ndII. apply (ndIE _ p).
+    { apply ndHI. now left. }
+    { apply ndHI. right. now left. }
   Qed.
 
 End implicative.
@@ -51,7 +49,6 @@ Section universals.
   Variable form : Type.
   Variable retract_univ : retract (form_univ form) form.
   Variable subst_form : (fin -> term) -> form -> form.
-  Variable retract_implicative : retract (form_implicative form) form.
 
   Variable count : form -> nat.
   Definition count_univ (p : form_univ form) : nat := match p with 
@@ -62,29 +59,21 @@ Section universals.
   Variable nd : list form -> form -> Prop.
 
   Definition up_ctx (A : list form) := map (subst_form (S >> var_term)) A.
-  Reserved Notation "A |- p" (at level 70).
   Inductive nd_univ (A : list form) : form -> Prop :=
-    | ndHU p : In p A -> A |- p
-    | ndUI p : up_ctx A |- p -> A |- ∀ p
-    | ndUE p t : A |- ∀ p -> A |- subst_form (t ..) p
-  where "A |- p" := (nd_univ A p).
+    | ndUI p : up_ctx A ⊢ p -> A ⊢ ∀ p
+    | ndUE p t : A ⊢ ∀ p -> A ⊢ subst_form (t ..) p
+  where "A ⊢ p" := (nd_univ A p).
 
-  Lemma weakening_univ A B p : A |- p -> incl A B -> B |- p.
+  Lemma weakening_univ A B p : A ⊢ p -> incl A B -> B ⊢ p.
   Proof. intro. revert B. induction H; intros B Hinc.
-    -apply ndHU. now apply Hinc.
     -apply ndUI, (IHnd_univ (up_ctx B)). unfold up_ctx. now apply incl_map.
     -apply ndUE. now apply IHnd_univ.
   Qed.
 
+  Variable retract_implicative : retract (form_implicative form) form.
   Variable equiv_nd : forall A p, nd_imp _ _ A p <-> nd_univ A p.
-  Lemma double_neg_univ A p : A |- p -> A |- ¬¬p.
-  Proof. induction 1; apply equiv_nd, ndII.
-    -apply (ndIE _ _ _ p). { apply ndHI. now left. } { apply ndHI. now right. }
-    -apply (ndIE _ _ _ (∀ p)). { apply ndHI. now left. }
-      { apply equiv_nd, ndUI, (weakening_univ (up_ctx A)). assumption.
-        unfold up_ctx. now apply incl_map, incl_tl. }
-    -apply (ndIE _ _ _ (subst_form (t ..) p)). { apply ndHI. now left. }
-      { apply equiv_nd, ndUE, (weakening_univ A). assumption. now apply incl_tl. }
+  Lemma double_neg_univ A (p : form) : A ⊢ p -> A ⊢ ¬¬( p).
+  Proof. intro. apply equiv_nd. apply (double_neg_imp _ _ A (p)). now apply equiv_nd.
   Qed.
 
 End universals.
@@ -95,18 +84,18 @@ Fixpoint count (p : form) := match p with
 end.
 
 Definition nd (A : list form) (p : form) : Prop := match p with
-  | In_form_implicative p => nd_imp _ _ A (In_form_implicative p)
-  | In_form_univ p => nd_univ _ subst_form _ A (In_form_univ p)
+  | In_form_implicative _ => nd_imp _ _ A p
+  | In_form_univ _ => nd_univ _ _ subst_form A p
 end.
-Notation "A |- p" := (nd A p) (at level 70).
+Notation "A ⊢ p" := (nd A p) (at level 70).
 
-Lemma weakening A B p : A |- p -> incl A B -> B |- p.
+Lemma weakening A B p : A ⊢ p -> incl A B -> B ⊢ p.
 Proof. destruct p.
   -apply weakening_imp.
   -apply weakening_univ.
 Qed.
 
-Lemma double_neg A p : A |- p -> A |- ¬¬p.
+Lemma double_neg A p : A ⊢ p -> A ⊢ ¬¬p.
 Proof. destruct p.
   -apply double_neg_imp.
   -Check double_neg_univ.
